theories/lang/lib/memcpy.v
@@ -21,16 +21,16 @@ Notation "e1 <-{ n ',Σ' i } ! e2" :=
 
 Lemma wp_memcpy `{!lrustGS Σ} E l1 l2 vl1 vl2 q (n : Z):
   Z.of_nat (length vl1) = n → Z.of_nat (length vl2) = n →
-  {{{ l1 ↦∗ vl1 ∗ l2 ↦∗{q} vl2 }}}
+  {{{ l1 ↦∗s vl1 ∗ l2 ↦∗s{q} vl2 }}}
     #l1 <-{n} !#l2 @ E
-  {{{ RET #☠; l1 ↦∗ vl2 ∗ l2 ↦∗{q} vl2 }}}.
+  {{{ RET #☠; l1 ↦∗s vl2 ∗ l2 ↦∗s{q} vl2 }}}.
 Proof.
   iIntros (Hvl1 Hvl2 Φ) "(Hl1 & Hl2) HΦ".
   iLöb as "IH" forall (n l1 l2 vl1 vl2 Hvl1 Hvl2). wp_rec. wp_op; case_bool_decide; wp_if.
   - iApply "HΦ". assert (n = O) by lia; subst.
     destruct vl1, vl2; try discriminate. by iFrame.
   - destruct vl1 as [|v1 vl1], vl2 as [|v2 vl2], n as [|n|]; try (discriminate || lia).
-    revert Hvl1 Hvl2. intros [= Hvl1] [= Hvl2]; rewrite !heap_mapsto_vec_cons. subst n.
+    revert Hvl1 Hvl2. intros [= Hvl1] [= Hvl2]; rewrite !heap_mapsto_vec_cons_s. subst n.
     iDestruct "Hl1" as "[Hv1 Hl1]". iDestruct "Hl2" as "[Hv2 Hl2]".
     Local Opaque Zminus.
     wp_read; wp_write. do 3 wp_op. iApply ("IH" with "[%] [%] Hl1 Hl2"); [lia..|].
